ExamplePwMgr.v
@@ -1,74 +1,166 @@
-Require Import Ascii FunctionApp List String.
+Require Import Ascii FunctionApp List Program.Basics String.
 Import ListNotations.
 
-Inductive uiInput :=
+Section ui.
+
+  Inductive uiInput :=
   | uiConsoleIn : string -> uiInput
   | uiDecrypted : string -> uiInput.
 
-Inductive uiOutput :=
-  | uiConsoleOut : string -> uiOutput
-  | uiEncrypt : string -> uiOutput.
+  Context (world : Type).
+  Context (consoleOut : string -> action world).
+  Context (encrypt : string -> action world).
 
-Fixpoint split (sep : ascii) (s : string) : list string :=
-  match s with
-    | EmptyString => nil
-    | String c s' =>
-      if ascii_dec c sep then EmptyString :: split sep s'
-      else match split sep s' with
-             | nil => [String c EmptyString]
-             | w :: ws => String c w :: ws
-           end
+  Fixpoint split (sep : ascii) (s : string) : list string :=
+    match s with
+      | EmptyString => nil
+      | String c s' =>
+        if ascii_dec c sep then EmptyString :: split sep s'
+        else match split sep s' with
+               | nil => [String c EmptyString]
+               | w :: ws => String c w :: ws
+             end
+    end.
+
+  Definition newline := "010"%char.
+
+  Definition dump (pws : list (string * string)) : string :=
+    fold_right append ""%string
+               (map (fun p => (fst p ++ " " ++ snd p ++ String newline "")%string) pws).
+
+  Fixpoint load (s : string) : list (string * string) :=
+    flat_map (fun l => match split " " l with
+                         | account :: password :: nil => [(account, password)]
+                         | _ => nil
+                       end)
+             (split newline s).
+
+  CoFixpoint uiLoop (pws : list (string * string)) :=
+    Step (fun i =>
+            match i with
+
+              | uiConsoleIn s =>
+                match split " " s with
+
+                  | "get"%string :: account :: nil =>
+                    match
+                      find (fun p => if string_dec account (fst p)
+                                     then true else false) pws
+                    with
+                      | None =>
+                        (consoleOut "account not found", uiLoop pws)
+                      | Some (_, password) =>
+                        (consoleOut password, uiLoop pws)
+                    end
+
+                  | "set"%string :: account :: password :: nil =>
+                    let pws' :=
+                        (account, password)
+                          :: filter (fun p => if string_dec account (fst p)
+                                              then false else true) pws
+                    in (encrypt (dump pws'), uiLoop pws')
+
+                  | _ =>
+                    (consoleOut "unrecognized command", uiLoop pws)
+
+                end
+
+              | uiDecrypted s =>
+                (id, uiLoop (load s))
+
+            end).
+
+  Definition ui := uiLoop nil.
+
+End ui.
+
+
+Section net.
+
+  Inductive netInput :=
+  | netReceived : string -> netInput
+  | netEncrypted : string -> netInput.
+
+  Context (world : Type).
+  Context (send : string -> action world).
+  Context (decrypt : string -> action world).
+
+  CoFixpoint net :=
+    Step (fun i =>
+            match i with
+              | netReceived s => (decrypt s, net)
+              | netEncrypted s => (send s, net)
+            end).
+
+End net.
+
+
+Definition getStep {input output} (p : process input output) :=
+  match p with
+    | Step f => f
   end.
 
-Definition newline := "010"%char.
 
-Definition dump (pws : list (string * string)) : string :=
-  fold_right append ""%string
-             (map (fun p => (fst p ++ " " ++ snd p ++ String newline "")%string) pws).
+Section pwMgr.
 
-Fixpoint load (s : string) : list (string * string) :=
-  flat_map (fun l => match split " " l with
-                       | account :: password :: nil => [(account, password)]
-                       | _ => nil
-                     end)
-           (split newline s).
+  Context (world : Type).
+  Context (consoleOut : string -> action world).
+  Context (send : string -> action world).
 
-CoFixpoint uiLoop (pws : list (string * string)) :=
-  Step (fun i =>
-          match i with
+  Inductive pwMgrMessage :=
+  | pwMgrEncrypt : string -> pwMgrMessage
+  | pwMgrDecrypt : string -> pwMgrMessage.
 
-            | uiConsoleIn s =>
-              match split " " s with
+  Inductive pwMgrInput :=
+  | pwMgrConsoleIn : string -> pwMgrInput
+  | pwMgrReceived : string -> pwMgrInput.
 
-                | "get"%string :: account :: nil =>
-                  match
-                    find (fun p => if string_dec account (fst p)
-                                   then true else false) pws
-                  with
-                    | None =>
-                      ([uiConsoleOut "account not found"], uiLoop pws)
-                    | Some (_, password) =>
-                      ([uiConsoleOut password], uiLoop pws)
-                  end
+  CoFixpoint pwMgrLoop ui net : stackProcess pwMgrMessage pwMgrInput world :=
+    Step (fun i =>
+            match i with
+              | inl (pwMgrEncrypt s) =>
+                (* TODO: crypto *)
+                let (a, net') := getStep net (netEncrypted s) in (a, pwMgrLoop ui net')
+              | inl (pwMgrDecrypt s) =>
+                (* TODO: crypto *)
+                let (a, ui') := getStep ui (uiDecrypted s) in (a, pwMgrLoop ui' net)
+              | inr (pwMgrConsoleIn s) =>
+                let (a, ui') := getStep ui (uiConsoleIn s) in (a, pwMgrLoop ui' net)
+              | inr (pwMgrReceived s) =>
+                let (a, net') := getStep net (netReceived s) in (a, pwMgrLoop ui net')
+            end).
 
-                | "set"%string :: account :: password :: nil =>
-                  let pws' :=
-                      (account, password)
-                        :: filter (fun p => if string_dec account (fst p)
-                                            then false else true) pws
-                  in ([uiEncrypt (dump pws')], uiLoop pws')
+  Definition
+    mkPwMgrStack
+    (ui :
+       forall {world'},
+         (string -> action world') ->
+         (string -> action world') ->
+         process uiInput world')
+    (net :
+       forall {world'},
+         (string -> action world') ->
+         (string -> action world') ->
+         process netInput world') :
+    stackProcess pwMgrMessage pwMgrInput world :=
+    pwMgrLoop
+      (ui
+         (fun s => stackLift (consoleOut s))
+         (fun s => stackPush (pwMgrEncrypt s)))
+      (net
+         (fun s => stackLift (send s))
+         (fun s => stackPush (pwMgrDecrypt s))).
 
-                | _ =>
-                  ([uiConsoleOut "unrecognized command"], uiLoop pws)
+  Definition pwMgrStack := mkPwMgrStack ui net.
 
-              end
+  Theorem pwMgrGood : emptiesStackForever pwMgrStack.
+    admit.
+  Qed.
 
-            | uiDecrypted s =>
-              ([], uiLoop (load s))
+  Definition pwMgr := runStackProcess pwMgrStack pwMgrGood.
 
-          end).
+End pwMgr.
 
-Definition ui := uiLoop nil.
 
 Require Import ExtrOcamlBasic ExtrOcamlString.
-Extraction "ExamplePwMgr" ui.
+Extraction "ExamplePwMgr" pwMgr.
