FunctionApp.v
@@ -1,8 +1,74 @@
 Section process.
-  Context {input output: Type}.
+  Context {input : Type}.
+  Context {world : Type}.
 
   CoInductive process :=
-  | Step : (input -> list output * process) -> process.
+  | Step : (input -> (world -> world) * process) -> process.
+
+  Definition action := world -> world.
+
+  Definition runStep wp i :=
+    match wp with
+      | (w, Step pf) => let (a, p') := pf i in (a w, p')
+    end.
 End process.
 
 Arguments process : clear implicits.
+Arguments action : clear implicits.
+
+
+Section stackProcess.
+
+  Context {message : Type}.
+  Context {input : Type}.
+  Context {world : Type}.
+
+  Definition stackWorld := (list message * action world)%type.
+  Definition stackProcess := process (message + input) stackWorld.
+
+  Definition stackPush (m : message) : action stackWorld :=
+    fun sw => let (ms, a) := sw in ((m :: ms)%list, a).
+  Definition stackLift (a : action world) : action stackWorld :=
+    fun sw => let (ms, a') := sw in (ms, fun w => a (a' w)).
+
+  Inductive emptiesStack :
+    stackWorld * stackProcess -> Prop :=
+  | stackEmpty p :
+      emptiesStack (nil, @id world, p)
+  | popsStack m ms a p :
+      emptiesStack (runStep (ms, a, p) (inl m)) ->
+      emptiesStack ((m :: ms)%list, a, p).
+
+  Fixpoint stepStackProcess swp (h : emptiesStack swp) : action world * stackProcess.
+  destruct swp as [[[ | m ms] a] p].
+  { exact (a, p). }
+  {
+    refine (stepStackProcess (runStep (ms, a, p) (inl m)) _).
+    inversion h; trivial.
+  }
+  Defined.
+
+  CoInductive emptiesStackForever : stackProcess -> Prop :=
+  | emptiesStackStep p h :
+      (forall (i : input),
+         emptiesStackForever (snd (stepStackProcess
+                                     (runStep (nil, @id world, p) (inr i)) (h i)))) ->
+      emptiesStackForever p.
+
+  CoFixpoint runStackProcess (p : stackProcess) (h : emptiesStackForever p) : process input world.
+  refine
+    (Step (fun i =>
+             let ap' :=
+                 stepStackProcess
+                   (runStep (nil, @id world, p) (inr i))
+                   match h with
+                     | emptiesStackStep _ h1 _ => h1 i
+                   end in
+             (fst ap', runStackProcess (snd ap') _))).
+  destruct h; eauto.
+  Defined.
+
+End stackProcess.
+
+Arguments stackWorld : clear implicits.
+Arguments stackProcess : clear implicits.
